src/cddl/pulse/CDDL.Pulse.AST.Parse.fst
@@ -1,7 +1,9 @@
 module CDDL.Pulse.AST.Parse
 include CDDL.Pulse.AST.Base
+include CDDL.Pulse.AST.Literal
 include CDDL.Pulse.AST.Parse.ElemType
 include CDDL.Pulse.Parse.ArrayGroup
+include CDDL.Pulse.Parse.MapGroup
 include CDDL.Pulse.AST.Types
 open Pulse.Lib.Pervasives
 module Cbor = CBOR.Spec.API.Format
@@ -17,16 +19,42 @@ type parse_env
 = (n: typ_name se.se_bound) -> impl_zero_copy_parse vmatch (sp_env.tp_spec_typ n).parser (r_env n).sem_rel
 
 [@@sem_attr]
+let ancillary_validate_env
+  (#cbor_t: Type)
+  (vmatch: perm -> cbor_t -> Cbor.cbor -> slprop)
+  (se: sem_env)
+= (t: typ) -> (t_wf: ast0_wf_typ t { spec_wf_typ se false t t_wf }) -> option (impl_typ vmatch (typ_sem se t))
+
+[@@sem_attr]
+let ancillary_validate_env_extend
+  (#cbor_t: Type)
+  (#vmatch: perm -> cbor_t -> Cbor.cbor -> slprop)
+  (#se: sem_env)
+  (env1: ancillary_validate_env vmatch se)
+  (se2: sem_env {
+    sem_env_included se se2
+  })
+: Tot (ancillary_validate_env vmatch se2)
+= fun t t_wf ->
+  if bounded_wf_typ se.se_bound t t_wf
+  then begin
+    (env1 t t_wf)
+  end
+  else None
+
+[@@sem_attr]
 let ancillary_parse_env
   (#cbor_t: Type)
   (vmatch: perm -> cbor_t -> Cbor.cbor -> slprop)
   (#cbor_array_iterator_t: Type0)
   (cbor_array_iterator_match: perm -> cbor_array_iterator_t -> list Cbor.cbor -> slprop)  
+  (#cbor_map_iterator_t: Type0)
+  (cbor_map_iterator_match: perm -> cbor_map_iterator_t -> list (Cbor.cbor & Cbor.cbor) -> slprop)
   (#se: sem_env)
   (#s_env: target_type_env se.se_bound)
   (r_env: rel_env s_env)
   (sp_env: spec_env se s_env.te_type)
-= (t: typ) -> (t_wf: ast0_wf_typ t { spec_wf_typ se true t t_wf }) -> option (impl_zero_copy_parse vmatch (spec_of_wf_typ sp_env t_wf).parser (impl_type_sem vmatch cbor_array_iterator_match r_env (target_type_of_wf_typ t_wf)).sem_rel)
+= (t: typ) -> (t_wf: ast0_wf_typ t { spec_wf_typ se true t t_wf }) -> option (impl_typ vmatch (typ_sem se t) & impl_zero_copy_parse vmatch (spec_of_wf_typ sp_env t_wf).parser (impl_type_sem vmatch cbor_array_iterator_match cbor_map_iterator_match r_env (target_type_of_wf_typ t_wf)).sem_rel)
 
 [@@sem_attr]
 let ancillary_parse_env_extend
@@ -34,11 +62,13 @@ let ancillary_parse_env_extend
   (#vmatch: perm -> cbor_t -> Cbor.cbor -> slprop)
   (#cbor_array_iterator_t: Type0)
   (#cbor_array_iterator_match: perm -> cbor_array_iterator_t -> list Cbor.cbor -> slprop)  
+  (#cbor_map_iterator_t: Type0)
+  (#cbor_map_iterator_match: perm -> cbor_map_iterator_t -> list (Cbor.cbor & Cbor.cbor) -> slprop)
   (#se: sem_env)
   (#s_env: target_type_env se.se_bound)
   (#r_env: rel_env s_env)
   (#sp_env: spec_env se s_env.te_type)
-  (env1: ancillary_parse_env vmatch cbor_array_iterator_match r_env sp_env)
+  (env1: ancillary_parse_env vmatch cbor_array_iterator_match cbor_map_iterator_match r_env sp_env)
   (#se2: sem_env)
   (#s_env2: target_type_env se2.se_bound)
   (r_env2: rel_env s_env2 {
@@ -47,7 +77,7 @@ let ancillary_parse_env_extend
   (sp_env2: spec_env se2 s_env2.te_type {
     spec_env_included sp_env sp_env2
   })
-: Tot (ancillary_parse_env vmatch cbor_array_iterator_match r_env2 sp_env2)
+: Tot (ancillary_parse_env vmatch cbor_array_iterator_match cbor_map_iterator_match r_env2 sp_env2)
 = fun t t_wf ->
   if bounded_wf_typ se.se_bound t t_wf
   then begin
@@ -61,11 +91,13 @@ let ancillary_parse_array_group_env
   (vmatch: perm -> cbor_t -> Cbor.cbor -> slprop)
   (#cbor_array_iterator_t: Type0)
   (cbor_array_iterator_match: perm -> cbor_array_iterator_t -> list Cbor.cbor -> slprop)  
+  (#cbor_map_iterator_t: Type0)
+  (cbor_map_iterator_match: perm -> cbor_map_iterator_t -> list (Cbor.cbor & Cbor.cbor) -> slprop)
   (#se: sem_env)
   (#s_env: target_type_env se.se_bound)
   (r_env: rel_env s_env)
   (sp_env: spec_env se s_env.te_type)
-= (t: group) -> (t_wf: ast0_wf_array_group t { spec_wf_array_group se t t_wf }) -> option (impl_array_group cbor_array_iterator_match (array_group_sem se t) & impl_zero_copy_array_group cbor_array_iterator_match (spec_of_wf_array_group sp_env t_wf).ag_parser (impl_type_sem vmatch cbor_array_iterator_match r_env (target_type_of_wf_array_group t_wf)).sem_rel)
+= (t: group) -> (t_wf: ast0_wf_array_group t { spec_wf_array_group se t t_wf }) -> option (impl_array_group cbor_array_iterator_match (array_group_sem se t) & impl_zero_copy_array_group cbor_array_iterator_match (spec_of_wf_array_group sp_env t_wf).ag_parser (impl_type_sem vmatch cbor_array_iterator_match cbor_map_iterator_match r_env (target_type_of_wf_array_group t_wf)).sem_rel)
 
 [@@sem_attr]
 let ancillary_parse_array_group_env_extend
@@ -73,11 +105,13 @@ let ancillary_parse_array_group_env_extend
   (#vmatch: perm -> cbor_t -> Cbor.cbor -> slprop)
   (#cbor_array_iterator_t: Type0)
   (#cbor_array_iterator_match: perm -> cbor_array_iterator_t -> list Cbor.cbor -> slprop)  
+  (#cbor_map_iterator_t: Type0)
+  (#cbor_map_iterator_match: perm -> cbor_map_iterator_t -> list (Cbor.cbor & Cbor.cbor) -> slprop)
   (#se: sem_env)
   (#s_env: target_type_env se.se_bound)
   (#r_env: rel_env s_env)
   (#sp_env: spec_env se s_env.te_type)
-  (env1: ancillary_parse_array_group_env vmatch cbor_array_iterator_match r_env sp_env)
+  (env1: ancillary_parse_array_group_env vmatch cbor_array_iterator_match cbor_map_iterator_match r_env sp_env)
   (#se2: sem_env)
   (#s_env2: target_type_env se2.se_bound)
   (r_env2: rel_env s_env2 {
@@ -86,7 +120,7 @@ let ancillary_parse_array_group_env_extend
   (sp_env2: spec_env se2 s_env2.te_type {
     spec_env_included sp_env sp_env2
   })
-: Tot (ancillary_parse_array_group_env vmatch cbor_array_iterator_match r_env2 sp_env2)
+: Tot (ancillary_parse_array_group_env vmatch cbor_array_iterator_match cbor_map_iterator_match r_env2 sp_env2)
 = fun t t_wf ->
   if bounded_wf_array_group se.se_bound t t_wf
   then begin
@@ -102,7 +136,7 @@ module SZ = FStar.SizeT
 
 noeq
 type ask_for =
-| AskForType: t: typ -> ast0_wf_typ t -> ask_for
+| AskForType: t: typ -> ast0_wf_typ t -> bool -> ask_for
 | AskForArrayGroup: t: group -> ast0_wf_array_group t -> ask_for
 
 let ask_for_spec
@@ -110,8 +144,12 @@ let ask_for_spec
   (a: ask_for)
 : Tot prop
 = match a with
-  | AskForType t t_wf -> spec_wf_typ se true t t_wf
+  | AskForType t t_wf guarded -> spec_wf_typ se guarded t t_wf
   | AskForArrayGroup t t_wf -> spec_wf_array_group se t t_wf
+
+#push-options "--z3rlimit 1024 --query_stats"
+
+#restart-solver
 
 [@@sem_attr]
 let rec impl_zero_copy_wf_type
@@ -127,13 +165,14 @@ let rec impl_zero_copy_wf_type
   (r_env: rel_env s_env)
   (sp_env: spec_env se s_env.te_type)
   (p_env: parse_env vmatch r_env sp_env)
-  (ancillary: ancillary_parse_env vmatch cbor_array_iterator_match r_env sp_env)
-  (ancillary_ag: ancillary_parse_array_group_env vmatch cbor_array_iterator_match r_env sp_env)
+  (ancillary_v: ancillary_validate_env vmatch se)
+  (ancillary: ancillary_parse_env vmatch cbor_array_iterator_match cbor_map_iterator_match r_env sp_env)
+  (ancillary_ag: ancillary_parse_array_group_env vmatch cbor_array_iterator_match cbor_map_iterator_match r_env sp_env)
   (#t: typ)
   (t_wf: ast0_wf_typ t {
     spec_wf_typ se true t t_wf /\ SZ.fits_u64
   })
-: Pure (either (impl_zero_copy_parse vmatch (spec_of_wf_typ sp_env t_wf).parser (impl_type_sem vmatch cbor_array_iterator_match r_env (target_type_of_wf_typ t_wf)).sem_rel) (ask_for))
+: Pure (either (impl_zero_copy_parse vmatch (spec_of_wf_typ sp_env t_wf).parser (impl_type_sem vmatch cbor_array_iterator_match cbor_map_iterator_match r_env (target_type_of_wf_typ t_wf)).sem_rel) (ask_for))
     (requires True)
     (ensures (fun res -> match res with
     | Inl _ -> True
@@ -142,9 +181,9 @@ let rec impl_zero_copy_wf_type
     (decreases t_wf)
 = match t_wf with
   | WfTRewrite _ _ s ->
-    impl_zero_copy_wf_type impl v_env r_env sp_env p_env ancillary ancillary_ag s
+    impl_zero_copy_wf_type impl v_env r_env sp_env p_env ancillary_v ancillary ancillary_ag s
   | WfTTagged tg _ s ->
-    begin match impl_zero_copy_wf_type impl v_env r_env sp_env p_env ancillary ancillary_ag s with
+    begin match impl_zero_copy_wf_type impl v_env r_env sp_env p_env ancillary_v ancillary ancillary_ag s with
     | Inr ask -> Inr ask
     | Inl p ->
       begin match tg with
@@ -153,17 +192,17 @@ let rec impl_zero_copy_wf_type
       end
     end
   | WfTChoice _ _ s1 s2 ->
-    begin match impl_zero_copy_wf_type impl v_env r_env sp_env p_env ancillary ancillary_ag s1 with
+    begin match impl_zero_copy_wf_type impl v_env r_env sp_env p_env ancillary_v ancillary ancillary_ag s1 with
     | Inr ask -> Inr ask
     | Inl p1 ->
-      begin match impl_zero_copy_wf_type impl v_env r_env sp_env p_env ancillary ancillary_ag s2 with
+      begin match impl_zero_copy_wf_type impl v_env r_env sp_env p_env ancillary_v ancillary ancillary_ag s2 with
       | Inr ask -> Inr ask
       | Inl p2 -> Inl (impl_zero_copy_choice (V.validate_typ impl v_env true _ s1) p1 p2)
       end
     end
   | WfTElem e -> Inl (impl_zero_copy_elem_type vmatch impl.cbor_get_major_type impl.cbor_destr_int64 impl.cbor_get_string impl.cbor_destr_simple e)
   | WfTDetCbor _ _ s ->
-    begin match impl_zero_copy_wf_type impl v_env r_env sp_env p_env ancillary ancillary_ag s with
+    begin match impl_zero_copy_wf_type impl v_env r_env sp_env p_env ancillary_v ancillary ancillary_ag s with
     | Inr ask -> Inr ask
     | Inl p ->
       Inl (impl_zero_copy_det_cbor impl.cbor_get_string impl.cbor_det_parse _ p)
@@ -177,11 +216,18 @@ let rec impl_zero_copy_wf_type
     then Inl (impl_copyful_pure_as_zero_copy (impl_copyful_int_range_uint64 impl.cbor_destr_int64 (U64.uint_to_t lo) (U64.uint_to_t hi)))
     else Inl (impl_copyful_pure_as_zero_copy (impl_copyful_int_range_int64 impl.cbor_get_major_type impl.cbor_destr_int64 (I64.int_to_t lo) (I64.int_to_t hi)))
   | WfTDef n -> Inl (p_env n)
-  | WfTArray _ _ -> admit ()
-  | WfTMap _ _ _ -> admit ()
+  | WfTArray _ s ->
+    begin match impl_zero_copy_wf_array_group impl v_env r_env sp_env p_env ancillary_v ancillary ancillary_ag s with
+    | Inr a -> Inr a
+    | Inl ps -> Inl (impl_zero_copy_array impl.cbor_array_iterator_init ps)
+    end
+  | WfTMap _ _ s ->
+    begin match impl_zero_copy_wf_map_group impl v_env r_env sp_env p_env ancillary_v ancillary ancillary_ag s with
+    | Inr a -> Inr a
+    | Inl ps -> Inl (impl_zero_copy_map ps ())
+    end
 
-[@@sem_attr]
-let rec impl_zero_copy_wf_array_group
+and impl_zero_copy_wf_array_group
   (#cbor_t #t2 #t_arr #t_map: Type0)
   (#vmatch: (perm -> cbor_t -> Cbor.cbor -> slprop))
   (#vmatch2: (perm -> t2 -> (Cbor.cbor & Cbor.cbor) -> slprop))
@@ -194,13 +240,14 @@ let rec impl_zero_copy_wf_array_group
   (r_env: rel_env s_env)
   (sp_env: spec_env se s_env.te_type)
   (p_env: parse_env vmatch r_env sp_env)
-  (ancillary: ancillary_parse_env vmatch cbor_array_iterator_match r_env sp_env)
-  (ancillary_ag: ancillary_parse_array_group_env vmatch cbor_array_iterator_match r_env sp_env)
+  (ancillary_v: ancillary_validate_env vmatch se)
+  (ancillary: ancillary_parse_env vmatch cbor_array_iterator_match cbor_map_iterator_match r_env sp_env)
+  (ancillary_ag: ancillary_parse_array_group_env vmatch cbor_array_iterator_match cbor_map_iterator_match r_env sp_env)
   (#t: group)
   (t_wf: ast0_wf_array_group t {
     spec_wf_array_group se t t_wf /\ SZ.fits_u64
   })
-: Pure (either (impl_zero_copy_array_group cbor_array_iterator_match (spec_of_wf_array_group sp_env t_wf).ag_parser (impl_type_sem vmatch cbor_array_iterator_match r_env (target_type_of_wf_array_group t_wf)).sem_rel) (ask_for))
+: Pure (either (impl_zero_copy_array_group cbor_array_iterator_match (spec_of_wf_array_group sp_env t_wf).ag_parser (impl_type_sem vmatch cbor_array_iterator_match cbor_map_iterator_match r_env (target_type_of_wf_array_group t_wf)).sem_rel) (ask_for))
     (requires True)
     (ensures (fun res -> match res with
     | Inl _ -> True
@@ -209,13 +256,13 @@ let rec impl_zero_copy_wf_array_group
     (decreases t_wf)
 = match t_wf with
   | WfAElem _ _ _ t_wf' ->
-    begin match impl_zero_copy_wf_type impl v_env r_env sp_env p_env ancillary ancillary_ag t_wf' with
+    begin match impl_zero_copy_wf_type impl v_env r_env sp_env p_env ancillary_v ancillary ancillary_ag t_wf' with
     | Inl pt ->
       Inl (impl_zero_copy_array_group_item impl.cbor_array_iterator_next pt)
     | Inr ask -> Inr ask
     end
   | WfAZeroOrOne _ t_wf' ->
-    begin match impl_zero_copy_wf_array_group impl v_env r_env sp_env p_env ancillary ancillary_ag t_wf' with
+    begin match impl_zero_copy_wf_array_group impl v_env r_env sp_env p_env ancillary_v ancillary ancillary_ag t_wf' with
     | Inr ask -> Inr ask
     | Inl pe ->
       Inl (impl_zero_copy_array_group_zero_or_one pe (V.validate_array_group impl v_env _ t_wf'))
@@ -233,22 +280,131 @@ let rec impl_zero_copy_wf_array_group
       end
     end
   | WfAConcat _ _ t_wf1 t_wf2 ->
-    begin match impl_zero_copy_wf_array_group impl v_env r_env sp_env p_env ancillary ancillary_ag t_wf1 with
+    begin match impl_zero_copy_wf_array_group impl v_env r_env sp_env p_env ancillary_v ancillary ancillary_ag t_wf1 with
     | Inr ask -> Inr ask
     | Inl pg1 ->
-      begin match impl_zero_copy_wf_array_group impl v_env r_env sp_env p_env ancillary ancillary_ag t_wf2 with
+      begin match impl_zero_copy_wf_array_group impl v_env r_env sp_env p_env ancillary_v ancillary ancillary_ag t_wf2 with
       | Inr ask -> Inr ask
       | Inl pg2 -> Inl (impl_zero_copy_array_group_concat impl.cbor_array_iterator_length impl.cbor_array_iterator_share impl.cbor_array_iterator_gather impl.cbor_array_iterator_truncate pg1 (V.validate_array_group impl v_env _ t_wf1) pg2 ())
       end
     end
   | WfAChoice _ _ t_wf1 t_wf2 ->
-    begin match impl_zero_copy_wf_array_group impl v_env r_env sp_env p_env ancillary ancillary_ag t_wf1 with
+    begin match impl_zero_copy_wf_array_group impl v_env r_env sp_env p_env ancillary_v ancillary ancillary_ag t_wf1 with
     | Inr ask -> Inr ask
     | Inl pg1 ->
-      begin match impl_zero_copy_wf_array_group impl v_env r_env sp_env p_env ancillary ancillary_ag t_wf2 with
+      begin match impl_zero_copy_wf_array_group impl v_env r_env sp_env p_env ancillary_v ancillary ancillary_ag t_wf2 with
       | Inr ask -> Inr ask
       | Inl pg2 -> Inl (impl_zero_copy_array_group_choice pg1 (V.validate_array_group impl v_env _ t_wf1) pg2)
       end
     end
   | WfARewrite _ _ t_wf2 ->
-    impl_zero_copy_wf_array_group impl v_env r_env sp_env p_env ancillary ancillary_ag t_wf2
+    impl_zero_copy_wf_array_group impl v_env r_env sp_env p_env ancillary_v ancillary ancillary_ag t_wf2
+
+and impl_zero_copy_wf_map_group
+  (#cbor_t #t2 #t_arr #t_map: Type0)
+  (#vmatch: (perm -> cbor_t -> Cbor.cbor -> slprop))
+  (#vmatch2: (perm -> t2 -> (Cbor.cbor & Cbor.cbor) -> slprop))
+  (#cbor_array_iterator_match: (perm -> t_arr -> list Cbor.cbor -> slprop))
+  (#cbor_map_iterator_match: (perm -> t_map -> list (Cbor.cbor & Cbor.cbor) -> slprop))
+  (impl: cbor_impl vmatch vmatch2 cbor_array_iterator_match cbor_map_iterator_match)
+  (#se: sem_env)
+  (v_env: V.validator_env vmatch se)
+  (#s_env: target_type_env se.se_bound)
+  (r_env: rel_env s_env)
+  (sp_env: spec_env se s_env.te_type)
+  (p_env: parse_env vmatch r_env sp_env)
+  (ancillary_v: ancillary_validate_env vmatch se)
+  (ancillary: ancillary_parse_env vmatch cbor_array_iterator_match cbor_map_iterator_match r_env sp_env)
+  (ancillary_ag: ancillary_parse_array_group_env vmatch cbor_array_iterator_match cbor_map_iterator_match r_env sp_env)
+  (#t: elab_map_group)
+  (t_wf: ast0_wf_parse_map_group t {
+    spec_wf_parse_map_group se t t_wf /\ SZ.fits_u64
+  })
+: Pure (either (impl_zero_copy_map_group vmatch (spec_of_wf_map_group sp_env t_wf).mg_parser (impl_type_sem vmatch cbor_array_iterator_match cbor_map_iterator_match r_env (target_type_of_wf_map_group t_wf)).sem_rel) (ask_for))
+    (requires True)
+    (ensures (fun res -> match res with
+    | Inl _ -> True
+    | Inr a -> ask_for_spec se a
+    ))
+    (decreases t_wf)
+= match t_wf with
+  | WfMChoice _ s1 _ s2 ->
+    begin match impl_zero_copy_wf_map_group impl v_env r_env sp_env p_env ancillary_v ancillary ancillary_ag s1 with
+    | Inr a -> Inr a
+    | Inl ps1 ->
+      begin match impl_zero_copy_wf_map_group impl v_env r_env sp_env p_env ancillary_v ancillary ancillary_ag s2 with
+      | Inr a -> Inr a
+      | Inl ps2 ->
+        Inl (impl_zero_copy_map_choice (V.validate_map_group impl v_env _ s1) ps1 ps2 ())
+      end
+    end
+  | WfMConcat _ s1 _ s2 ->
+    begin match impl_zero_copy_wf_map_group impl v_env r_env sp_env p_env ancillary_v ancillary ancillary_ag s1 with
+    | Inr a -> Inr a
+    | Inl ps1 ->
+      begin match impl_zero_copy_wf_map_group impl v_env r_env sp_env p_env ancillary_v ancillary ancillary_ag s2 with
+      | Inr a -> Inr a
+      | Inl ps2 ->
+        Inl (impl_zero_copy_map_concat impl.cbor_share impl.cbor_gather ps1 ps2 ())
+      end
+    end
+  | WfMZeroOrOne _ s1 ->
+    begin match impl_zero_copy_wf_map_group impl v_env r_env sp_env p_env ancillary_v ancillary ancillary_ag s1 with
+    | Inr a -> Inr a
+    | Inl ps1 ->
+      Inl
+        (impl_zero_copy_map_ext
+          (impl_zero_copy_map_zero_or_one (V.validate_map_group impl v_env _ s1) ps1 ())
+          #_ #_ #(spec_of_wf_map_group sp_env t_wf).mg_size #(spec_of_wf_map_group sp_env t_wf).mg_serializable
+          (spec_of_wf_map_group sp_env t_wf).mg_parser
+          ()
+        )
+    end
+  | WfMLiteral cut key _ s ->
+    begin match impl_zero_copy_wf_type impl v_env r_env sp_env p_env ancillary_v ancillary ancillary_ag s with
+    | Inr a -> Inr a
+    | Inl ps1 ->
+      Inl
+        (impl_zero_copy_match_item_for
+          impl.cbor_map_get
+          (with_literal
+            impl.cbor_mk_int64
+            impl.cbor_elim_int64
+            impl.cbor_mk_simple
+            impl.cbor_elim_simple
+            impl.cbor_mk_string
+            key
+          )
+          cut
+          ps1
+        )
+    end
+  | WfMZeroOrMore _ _ _ s_key s_key_except s_value ->
+    begin match ancillary _ s_key with
+    | None -> Inr (AskForType _ s_key true)
+    | Some (v_key, p_key) ->
+      begin match ancillary_v _ s_key_except with
+      | None -> Inr (AskForType _ s_key_except false)
+      | Some (v_key_except) ->
+        begin match ancillary _ s_value with
+        | None -> Inr (AskForType _ s_value true)
+        | Some (v_value, p_value) ->
+          Inl
+            (impl_zero_copy_map_zero_or_more
+              impl.cbor_map_iterator_init
+              impl.cbor_map_iterator_share
+              impl.cbor_map_iterator_gather
+              (target_type_eq s_env (target_type_of_wf_typ s_key))
+              (spec_of_wf_typ sp_env s_key)
+              v_key
+              p_key
+              v_key_except
+              (spec_of_wf_typ sp_env s_value)
+              v_value
+              p_value
+            )
+        end
+      end
+    end
+
+#pop-options
